src/JSON/Utils/Unicode.dfy
@@ -1,6 +1,6 @@
-include "../BoundedInts.dfy"
+include "../../BoundedInts.dfy"
 
-module {:options "/functionSyntax:4"} JSON.Unicode {
+module {:options "/functionSyntax:4"} JSON.Utils.Unicode {
   import opened BoundedInts
 
   function Utf16Decode1(c: uint16): uint32
